@prefix skos: <http://www.w3.org/2004/02/skos/core#> .

<https://vocab.sentier.dev/products/aec-electrolyzer> a skos:Concept ;
    skos:broader "https://vocab.sentier.dev/products/electrolyzer" ;
    skos:broaderTransitive "https://vocab.sentier.dev/products/electrolyzer" ;
    skos:definition "An electrolyser with two electrodes operating in a liquid alkaline electrolyte."@en ;
    skos:prefLabel "Alkaline Electrolysis Cell Electrolyzer"@en ;
    skos:related <https://en.wikipedia.org/wiki/Alkaline_water_electrolysis> .

<https://vocab.sentier.dev/products/electrolyzer> a skos:Concept ;
    skos:broader "http://data.europa.eu/xsp/cn2024/854330700080" ;
    skos:broaderTransitive "http://data.europa.eu/xsp/cn2024/854330700080" ;
    skos:definition "An electrolyzer is a machine that uses electricity to drive a chemical reaction."@en ;
    skos:prefLabel "Electrolyzer"@en-GB,
        "Electrolyzer"@en-US ;
    skos:related <https://en.wikipedia.org/wiki/Electrolysis> .

<https://vocab.sentier.dev/products/pem-electrolyzer> a skos:Concept ;
    skos:broader "https://vocab.sentier.dev/products/electrolyzer" ;
    skos:broaderTransitive "https://vocab.sentier.dev/products/electrolyzer" ;
    skos:definition "An electrolyser with a solid polymer electrolyte and a proton exchange membrane."@en ;
    skos:prefLabel "Proton Exchange Membrane Electrolyser"@en-GB,
        "Proton Exchange Membrane Electrolyzer"@en-US ;
    skos:related <https://en.wikipedia.org/wiki/Proton_exchange_membrane_electrolysis> .

<https://vocab.sentier.dev/products/soel-electrolyzer> a skos:Concept ;
    skos:broader "https://vocab.sentier.dev/products/electrolyzer" ;
    skos:broaderTransitive "https://vocab.sentier.dev/products/electrolyzer" ;
    skos:definition "A solid oxide fuel cell that runs in regenerative mode to achieve the electrolysis of water."@en ;
    skos:prefLabel "Solid Oxide Electrolyzer"@en ;
    skos:related <https://en.wikipedia.org/wiki/Solid_oxide_electrolyzer_cell> .

<https://vocab.sentier.dev/products/tetrafluoroethylene> a skos:Concept ;
    skos:broader "http://data.europa.eu/xsp/cn2024/290349000080" ;
    skos:broaderTransitive "http://data.europa.eu/xsp/cn2024/290349000080" ;
    skos:definition "Tetrafluoroethylene (TFE) is a fluorocarbon with the chemical formula C2F4. It is the simplest perfluorinated alkene. This gaseous species is used primarily in the industrial preparation of fluoropolymers (from Wikipedia)"@en ;
    skos:prefLabel "Tetrafluoroethylene"@en ;
    skos:related <https://en.wikipedia.org/wiki/Tetrafluoroethylene> .

<https://vocab.sentier.dev/products/zeolite> a skos:Concept ;
    skos:broader "http://data.europa.eu/xsp/cn2024/382400000080" ;
    skos:broaderTransitive "http://data.europa.eu/xsp/cn2024/382400000080" ;
    skos:definition "Zeolite is a family of several microporous, crystalline aluminosilicate materials commonly used as commercial adsorbents and catalysts (from Wikipedia)"@en ;
    skos:prefLabel "Zeolite"@en ;
    skos:related <https://en.wikipedia.org/wiki/Zeolite> .

"http://data.europa.eu/xsp/cn2024/290349000080" skos:narrower <https://vocab.sentier.dev/products/tetrafluoroethylene> ;
    skos:narrowerTransitive <https://vocab.sentier.dev/products/tetrafluoroethylene> .

"http://data.europa.eu/xsp/cn2024/382400000080" skos:narrower <https://vocab.sentier.dev/products/zeolite> ;
    skos:narrowerTransitive <https://vocab.sentier.dev/products/zeolite> .

"http://data.europa.eu/xsp/cn2024/854330700080" skos:narrower <https://vocab.sentier.dev/products/electrolyzer> ;
    skos:narrowerTransitive <https://vocab.sentier.dev/products/electrolyzer> .

"https://vocab.sentier.dev/products/electrolyzer" skos:narrower <https://vocab.sentier.dev/products/aec-electrolyzer>,
        <https://vocab.sentier.dev/products/pem-electrolyzer>,
        <https://vocab.sentier.dev/products/soel-electrolyzer> ;
    skos:narrowerTransitive <https://vocab.sentier.dev/products/aec-electrolyzer>,
        <https://vocab.sentier.dev/products/pem-electrolyzer>,
        <https://vocab.sentier.dev/products/soel-electrolyzer> .

