@prefix skos: <http://www.w3.org/2004/02/skos/core#> .

<https://vocab.sentier.dev/products/electricity/biomass> a skos:Concept ;
    skos:broader <https://vocab.sentier.dev/products/electricity/other-renewable> ;
    skos:broaderTransitive <http://openenergy-platform.org/ontology/oeo/OEO_00010384>,
        <https://vocab.sentier.dev/products/electricity/other-renewable> ;
    skos:definition "Electrical energy from biomass is generated by burning organic materials such as plant and animal waste to produce electricity."@en ;
    skos:prefLabel "Electrical energy from biomass"@en ;
    skos:related <https://en.wikipedia.org/wiki/Bioenergy> .

<https://vocab.sentier.dev/products/electricity/coalbed-gas> a skos:Concept ;
    skos:broader <https://vocab.sentier.dev/products/electricity/fossil-gas> ;
    skos:broaderTransitive <http://data.europa.eu/xsp/cn2024/271600000080>,
        <https://vocab.sentier.dev/products/electricity/fossil-fuel>,
        <https://vocab.sentier.dev/products/electricity/fossil-gas> ;
    skos:definition "Electrical energy from coal seam gas is generated through the combustion of coal seam gas."@en ;
    skos:prefLabel "Electrical energy from coal seam gas"@en ;
    skos:related <https://en.wikipedia.org/wiki/Coalbed_methane> .

<https://vocab.sentier.dev/products/electricity/crude-oil> a skos:Concept ;
    skos:broader <https://vocab.sentier.dev/products/electricity/fossil-oil> ;
    skos:broaderTransitive <https://vocab.sentier.dev/products/electricity/fossil-energy>,
        <https://vocab.sentier.dev/products/electricity/fossil-oil> ;
    skos:definition "Electrical energy from crude oil refers to electricity generated from the combustion of crude oil."@en ;
    skos:prefLabel "Electrical energy from crude oil"@en ;
    skos:related <https://en.wikipedia.org/wiki/Petroleum> .

<https://vocab.sentier.dev/products/electricity/fossil-coal> a skos:Concept ;
    skos:broader <https://vocab.sentier.dev/products/electricity/fossil-fuel> ;
    skos:broaderTransitive <http://data.europa.eu/xsp/cn2024/271600000080>,
        <https://vocab.sentier.dev/products/electricity/fossil-fuel> ;
    skos:definition "Coal-based electrical energy is electrical energy produced by the combustion of coal."@en ;
    skos:narrower <https://vocab.sentier.dev/products/electricity/hard-coal>,
        <https://vocab.sentier.dev/products/electricity/lignite> ;
    skos:narrowerTransitive <https://vocab.sentier.dev/products/electricity/hard-coal>,
        <https://vocab.sentier.dev/products/electricity/lignite> ;
    skos:prefLabel "Coal-based electrical energy"@en ;
    skos:related <https://en.wikipedia.org/wiki/Coal-fired_power_station> .

<https://vocab.sentier.dev/products/electricity/fossil-fuel> a skos:Concept ;
    skos:broader <http://data.europa.eu/xsp/cn2024/271600000080> ;
    skos:broaderTransitive <http://data.europa.eu/xsp/cn2024/271600000080> ;
    skos:definition "Fossil fuel-based electrical energy is electrical energy produced by incineration of fossil fuels."@en ;
    skos:narrower <https://vocab.sentier.dev/products/electricity/fossil-coal>,
        <https://vocab.sentier.dev/products/electricity/fossil-gas>,
        <https://vocab.sentier.dev/products/electricity/peat> ;
    skos:narrowerTransitive <https://vocab.sentier.dev/products/electricity/coalbed-gas>,
        <https://vocab.sentier.dev/products/electricity/fossil-coal>,
        <https://vocab.sentier.dev/products/electricity/fossil-gas>,
        <https://vocab.sentier.dev/products/electricity/hard-coal>,
        <https://vocab.sentier.dev/products/electricity/lignite>,
        <https://vocab.sentier.dev/products/electricity/natural-gas>,
        <https://vocab.sentier.dev/products/electricity/peat> ;
    skos:prefLabel "Fossil fuel-based electrical energy"@en ;
    skos:related <https://en.wikipedia.org/wiki/Fossil_fuel> .

<https://vocab.sentier.dev/products/electricity/fossil-gas> a skos:Concept ;
    skos:broader <https://vocab.sentier.dev/products/electricity/fossil-fuel> ;
    skos:broaderTransitive <http://data.europa.eu/xsp/cn2024/271600000080>,
        <https://vocab.sentier.dev/products/electricity/fossil-fuel> ;
    skos:definition "Natural gas-based electrical energy is electrical energy produced through the combustion of natural gas."@en ;
    skos:narrower <https://vocab.sentier.dev/products/electricity/coalbed-gas>,
        <https://vocab.sentier.dev/products/electricity/natural-gas> ;
    skos:narrowerTransitive <https://vocab.sentier.dev/products/electricity/coalbed-gas>,
        <https://vocab.sentier.dev/products/electricity/natural-gas> ;
    skos:prefLabel "Natural gas-based electrical energy"@en ;
    skos:related <https://en.wikipedia.org/wiki/Natural_gas> .

<https://vocab.sentier.dev/products/electricity/fossil-oil> a skos:Concept ;
    skos:broader <https://vocab.sentier.dev/products/electricity/fossil-energy> ;
    skos:broaderTransitive <https://vocab.sentier.dev/products/electricity/fossil-energy> ;
    skos:definition "Fossil oil-based electrical energy is electrical energy produced by the combustion of fossil oils."@en ;
    skos:narrower <https://vocab.sentier.dev/products/electricity/crude-oil>,
        <https://vocab.sentier.dev/products/electricity/oil-shale> ;
    skos:narrowerTransitive <https://vocab.sentier.dev/products/electricity/crude-oil>,
        <https://vocab.sentier.dev/products/electricity/oil-shale> ;
    skos:prefLabel "Fossil oil-based electrical energy"@en ;
    skos:related <https://en.wikipedia.org/wiki/Petroleum> .

<https://vocab.sentier.dev/products/electricity/geothermal> a skos:Concept ;
    skos:broader <https://vocab.sentier.dev/products/electricity/other-renewable> ;
    skos:broaderTransitive <http://openenergy-platform.org/ontology/oeo/OEO_00010384>,
        <https://vocab.sentier.dev/products/electricity/other-renewable> ;
    skos:definition "Electrical energy from geothermal sources is generated by harnessing heat from the earth's interior."@en ;
    skos:prefLabel "Electrical energy from geothermal sources"@en ;
    skos:related <https://en.wikipedia.org/wiki/Geothermal_energy> .

<https://vocab.sentier.dev/products/electricity/hard-coal> a skos:Concept ;
    skos:broader <https://vocab.sentier.dev/products/electricity/fossil-coal> ;
    skos:broaderTransitive <http://data.europa.eu/xsp/cn2024/271600000080>,
        <https://vocab.sentier.dev/products/electricity/fossil-coal>,
        <https://vocab.sentier.dev/products/electricity/fossil-fuel> ;
    skos:definition "Electrical energy from hard coal is generated from the combustion of hard coal."@en ;
    skos:prefLabel "Electrical energy from hard coal"@en ;
    skos:related <https://en.wikipedia.org/wiki/Coal-fired_power_station> .

<https://vocab.sentier.dev/products/electricity/hydro-reservoirs> a skos:Concept ;
    skos:broader <https://vocab.sentier.dev/products/electricity/hydropower> ;
    skos:broaderTransitive <http://openenergy-platform.org/ontology/oeo/OEO_00010384>,
        <https://vocab.sentier.dev/products/electricity/hydropower> ;
    skos:definition "Electrical energy from hydro water reservoirs is generated using stored water in reservoirs to drive hydro turbines."@en ;
    skos:prefLabel "Electrical energy from hydro water reservoirs"@en ;
    skos:related <https://en.wikipedia.org/wiki/Reservoir> .

<https://vocab.sentier.dev/products/electricity/hydropower> a skos:Concept ;
    skos:broader <http://openenergy-platform.org/ontology/oeo/OEO_00010384> ;
    skos:broaderTransitive <http://openenergy-platform.org/ontology/oeo/OEO_00010384> ;
    skos:definition "Electricity from hydropower is electrical energy generated through the use of water resources."@en ;
    skos:narrower <https://vocab.sentier.dev/products/electricity/hydro-reservoirs>,
        <https://vocab.sentier.dev/products/electricity/marine>,
        <https://vocab.sentier.dev/products/electricity/pumped-storage>,
        <https://vocab.sentier.dev/products/electricity/run-of-river> ;
    skos:narrowerTransitive <https://vocab.sentier.dev/products/electricity/hydro-reservoirs>,
        <https://vocab.sentier.dev/products/electricity/marine>,
        <https://vocab.sentier.dev/products/electricity/pumped-storage>,
        <https://vocab.sentier.dev/products/electricity/run-of-river> ;
    skos:prefLabel "Electricity from hydropower"@en ;
    skos:related <https://en.wikipedia.org/wiki/Hydroelectricity> .

<https://vocab.sentier.dev/products/electricity/lignite> a skos:Concept ;
    skos:broader <https://vocab.sentier.dev/products/electricity/fossil-coal> ;
    skos:broaderTransitive <http://data.europa.eu/xsp/cn2024/271600000080>,
        <https://vocab.sentier.dev/products/electricity/fossil-coal>,
        <https://vocab.sentier.dev/products/electricity/fossil-fuel> ;
    skos:definition "Electrical energy from brown coal/lignite is generated from the combustion of brown coal or lignite."@en ;
    skos:prefLabel "Electrical energy from brown coal/lignite"@en ;
    skos:related <https://en.wikipedia.org/wiki/Lignite> .

<https://vocab.sentier.dev/products/electricity/marine> a skos:Concept ;
    skos:broader <https://vocab.sentier.dev/products/electricity/hydropower> ;
    skos:broaderTransitive <http://openenergy-platform.org/ontology/oeo/OEO_00010384>,
        <https://vocab.sentier.dev/products/electricity/hydropower> ;
    skos:definition "Electrical energy from marine sources is generated from ocean and tidal forces, exploiting kinetic energy."@en ;
    skos:prefLabel "Electrical energy from marine sources"@en ;
    skos:related <https://en.wikipedia.org/wiki/Marine_energy> .

<https://vocab.sentier.dev/products/electricity/natural-gas> a skos:Concept ;
    skos:broader <https://vocab.sentier.dev/products/electricity/fossil-gas> ;
    skos:broaderTransitive <http://data.europa.eu/xsp/cn2024/271600000080>,
        <https://vocab.sentier.dev/products/electricity/fossil-fuel>,
        <https://vocab.sentier.dev/products/electricity/fossil-gas> ;
    skos:definition "Electrical energy from natural gas refers to electricity generated from the combustion of natural gas."@en ;
    skos:prefLabel "Electrical energy from natural gas"@en ;
    skos:related <https://en.wikipedia.org/wiki/Natural_gas> .

<https://vocab.sentier.dev/products/electricity/offshore> a skos:Concept ;
    skos:broader <https://vocab.sentier.dev/products/electricity/wind-energy> ;
    skos:broaderTransitive <http://openenergy-platform.org/ontology/oeo/OEO_00010384>,
        <https://vocab.sentier.dev/products/electricity/wind-energy> ;
    skos:definition "Electrical energy from offshore wind is generated by wind turbines located in bodies of water."@en ;
    skos:prefLabel "Electricity from offshore wind energy"@en ;
    skos:related <https://en.wikipedia.org/wiki/Offshore_wind_power> .

<https://vocab.sentier.dev/products/electricity/oil-shale> a skos:Concept ;
    skos:broader <https://vocab.sentier.dev/products/electricity/fossil-oil> ;
    skos:broaderTransitive <https://vocab.sentier.dev/products/electricity/fossil-energy>,
        <https://vocab.sentier.dev/products/electricity/fossil-oil> ;
    skos:definition "Electrical energy from oil shale is generated from the processing and combustion of oil shale."@en ;
    skos:prefLabel "Electrical energy from oil shale"@en ;
    skos:related <https://en.wikipedia.org/wiki/Oil_shale> .

<https://vocab.sentier.dev/products/electricity/onshore> a skos:Concept ;
    skos:broader <https://vocab.sentier.dev/products/electricity/wind-energy> ;
    skos:broaderTransitive <http://openenergy-platform.org/ontology/oeo/OEO_00010384>,
        <https://vocab.sentier.dev/products/electricity/wind-energy> ;
    skos:definition "Electricity from onshore wind energy is generated by wind turbines located on land."@en ;
    skos:prefLabel "Electricity from onshore wind energy"@en ;
    skos:related <https://en.wikipedia.org/wiki/Wind_power> .

<https://vocab.sentier.dev/products/electricity/other> a skos:Concept ;
    skos:broader <http://data.europa.eu/xsp/cn2024/271600000080> ;
    skos:broaderTransitive <http://data.europa.eu/xsp/cn2024/271600000080> ;
    skos:definition "Other electrical energy includes various forms of electrical energy generation not classified as renewable or fossil fuel-based."@en ;
    skos:prefLabel "Other electrical energy"@en .

<https://vocab.sentier.dev/products/electricity/other-renewable> a skos:Concept ;
    skos:broader <http://openenergy-platform.org/ontology/oeo/OEO_00010384> ;
    skos:broaderTransitive <http://openenergy-platform.org/ontology/oeo/OEO_00010384> ;
    skos:definition "Other renewable electrical energy includes electricity generated from sources such as geothermal and biomass."@en ;
    skos:narrower <https://vocab.sentier.dev/products/electricity/biomass>,
        <https://vocab.sentier.dev/products/electricity/geothermal>,
        <https://vocab.sentier.dev/products/electricity/other-renewable-sources> ;
    skos:narrowerTransitive <https://vocab.sentier.dev/products/electricity/biomass>,
        <https://vocab.sentier.dev/products/electricity/geothermal>,
        <https://vocab.sentier.dev/products/electricity/other-renewable-sources> ;
    skos:prefLabel "Other renewable electrical energy"@en .

<https://vocab.sentier.dev/products/electricity/other-renewable-sources> a skos:Concept ;
    skos:broader <https://vocab.sentier.dev/products/electricity/other-renewable> ;
    skos:broaderTransitive <http://openenergy-platform.org/ontology/oeo/OEO_00010384>,
        <https://vocab.sentier.dev/products/electricity/other-renewable> ;
    skos:definition "Electrical energy from other renewable sources includes electricity generated from various innovative renewable technologies."@en ;
    skos:prefLabel "Electrical energy from other renewable sources"@en-US .

<https://vocab.sentier.dev/products/electricity/peat> a skos:Concept ;
    skos:broader <https://vocab.sentier.dev/products/electricity/fossil-fuel> ;
    skos:broaderTransitive <http://data.europa.eu/xsp/cn2024/271600000080>,
        <https://vocab.sentier.dev/products/electricity/fossil-fuel> ;
    skos:definition "Electrical energy from peat is generated through the combustion of peat."@en ;
    skos:prefLabel "Electrical energy from peat"@en ;
    skos:related <https://en.wikipedia.org/wiki/Peat> .

<https://vocab.sentier.dev/products/electricity/pumped-storage> a skos:Concept ;
    skos:broader <https://vocab.sentier.dev/products/electricity/hydropower> ;
    skos:broaderTransitive <http://openenergy-platform.org/ontology/oeo/OEO_00010384>,
        <https://vocab.sentier.dev/products/electricity/hydropower> ;
    skos:definition "Electrical energy from pumped storage hydro is generated through a two-reservoir system where water is pumped to a higher elevation for storage and released to generate electricity."@en ;
    skos:prefLabel "Electrical energy from pumped storage hydro"@en ;
    skos:related <https://en.wikipedia.org/wiki/Pumped-storage_hydroelectricity> .

<https://vocab.sentier.dev/products/electricity/run-of-river> a skos:Concept ;
    skos:broader <https://vocab.sentier.dev/products/electricity/hydropower> ;
    skos:broaderTransitive <http://openenergy-platform.org/ontology/oeo/OEO_00010384>,
        <https://vocab.sentier.dev/products/electricity/hydropower> ;
    skos:definition "Electrical energy from run-of-river and poundage hydro is generated without large reservoirs, utilizing the natural flow of rivers."@en ;
    skos:prefLabel "Electrical energy from run-of-river and poundage hydro"@en ;
    skos:related <https://en.wikipedia.org/wiki/Run-of-the-river_hydroelectricity> .

<https://vocab.sentier.dev/products/electricity/waste> a skos:Concept ;
    skos:broader <http://data.europa.eu/xsp/cn2024/271600000080> ;
    skos:broaderTransitive <http://data.europa.eu/xsp/cn2024/271600000080> ;
    skos:definition "Waste-based electrical energy is generated by converting waste materials into electricity, typically through incineration or anaerobic digestion."@en ;
    skos:prefLabel "Waste-based electrical energy"@en-US ;
    skos:related <https://en.wikipedia.org/wiki/Waste-to-energy> .

<https://vocab.sentier.dev/products/electricity/wind-energy> a skos:Concept ;
    skos:broader <http://openenergy-platform.org/ontology/oeo/OEO_00010384> ;
    skos:broaderTransitive <http://openenergy-platform.org/ontology/oeo/OEO_00010384> ;
    skos:definition "Electricity from wind energy is electrical energy produced by converting wind energy into electricity through wind turbines."@en ;
    skos:narrower <https://vocab.sentier.dev/products/electricity/offshore>,
        <https://vocab.sentier.dev/products/electricity/onshore> ;
    skos:narrowerTransitive <https://vocab.sentier.dev/products/electricity/offshore>,
        <https://vocab.sentier.dev/products/electricity/onshore> ;
    skos:prefLabel "Electricity from wind energy"@en ;
    skos:related <https://en.wikipedia.org/wiki/Wind_power> .

<https://vocab.sentier.dev/products/electricity/fossil-energy> skos:narrower <https://vocab.sentier.dev/products/electricity/fossil-oil> ;
    skos:narrowerTransitive <https://vocab.sentier.dev/products/electricity/crude-oil>,
        <https://vocab.sentier.dev/products/electricity/fossil-oil>,
        <https://vocab.sentier.dev/products/electricity/oil-shale> .

<http://data.europa.eu/xsp/cn2024/271600000080> skos:narrower <https://vocab.sentier.dev/products/electricity/fossil-fuel>,
        <https://vocab.sentier.dev/products/electricity/other>,
        <https://vocab.sentier.dev/products/electricity/waste> ;
    skos:narrowerTransitive <https://vocab.sentier.dev/products/electricity/coalbed-gas>,
        <https://vocab.sentier.dev/products/electricity/fossil-coal>,
        <https://vocab.sentier.dev/products/electricity/fossil-fuel>,
        <https://vocab.sentier.dev/products/electricity/fossil-gas>,
        <https://vocab.sentier.dev/products/electricity/hard-coal>,
        <https://vocab.sentier.dev/products/electricity/lignite>,
        <https://vocab.sentier.dev/products/electricity/natural-gas>,
        <https://vocab.sentier.dev/products/electricity/other>,
        <https://vocab.sentier.dev/products/electricity/peat>,
        <https://vocab.sentier.dev/products/electricity/waste> .

<http://openenergy-platform.org/ontology/oeo/OEO_00010384> skos:narrower <https://vocab.sentier.dev/products/electricity/hydropower>,
        <https://vocab.sentier.dev/products/electricity/other-renewable>,
        <https://vocab.sentier.dev/products/electricity/wind-energy> ;
    skos:narrowerTransitive <https://vocab.sentier.dev/products/electricity/biomass>,
        <https://vocab.sentier.dev/products/electricity/geothermal>,
        <https://vocab.sentier.dev/products/electricity/hydro-reservoirs>,
        <https://vocab.sentier.dev/products/electricity/hydropower>,
        <https://vocab.sentier.dev/products/electricity/marine>,
        <https://vocab.sentier.dev/products/electricity/offshore>,
        <https://vocab.sentier.dev/products/electricity/onshore>,
        <https://vocab.sentier.dev/products/electricity/other-renewable>,
        <https://vocab.sentier.dev/products/electricity/other-renewable-sources>,
        <https://vocab.sentier.dev/products/electricity/pumped-storage>,
        <https://vocab.sentier.dev/products/electricity/run-of-river>,
        <https://vocab.sentier.dev/products/electricity/wind-energy> .

